2020/day18/Part1.fst
@@ -2,44 +2,87 @@ module Part1
 
 open Parser
 open FStar.String
+open FStar.Printf
 open FStar.IO
 open FStar.All
 
-(*
 type ast =
   | Number : n:int -> ast
   | Add : left:ast -> right:ast -> ast
   | Mul : left:ast -> right:ast -> ast
+  | Paren : inner:ast -> ast
 
-*)
-(*
+let rec print_ast (indent:string) (x:ast) : ML unit =
+  match x with 
+  | Number n -> print_string (sprintf "%s%d\n" indent n)
+  | Add left right -> 
+      print_string (indent ^ "(+\n");
+      print_ast (indent ^ "  ") left;
+      print_ast (indent ^ "  ") right;
+      print_string (indent ^ ")\n")
+  | Mul left right -> 
+      print_string (indent ^ "(*\n");
+      print_ast (indent ^ "  ") left;
+      print_ast (indent ^ "  ") right;
+      print_string (indent ^ ")\n")
+  | Paren inner -> 
+     print_string (indent ^ "[\n");
+      print_ast (indent ^ "  ") inner;
+      print_string (indent ^ "]\n")
+      
 let parse_number : parser ast =
   space (parse_apply (fun z -> Number z) unsigned_integer )
- *)
 
-let rec parse_recursive (input:string) : Tot (parse_result string input) (decreases strlen(input)) =
-    (parse_either_ctx input
-      (parse_forget (literal_char 'x'))
-      (brackets_char input '(' parse_recursive ')'))
-      input
+let token_plus : parser string =
+  space (parse_forget (literal_char '+'))
 
-let parse_or_report_fail (x:(parser string)) : ML unit =
+let token_star : parser string =
+  space (parse_forget (literal_char '*'))
+
+let rec parse_ast (input:string) : Tot (parse_result ast input) (decreases (strlen input)) =
+  parse_alternatives_ctx input
+    [
+      // These are tried in-order; we can't recurse into ast directly
+      // ( ast ) + ast
+      (binop_char_ctxe input 
+         (brackets_char input '(' parse_ast ')' )
+         token_plus 
+         (space_ctx input parse_ast)
+         (fun left right -> Add (Paren left) right));
+      // ( ast ) * ast
+      (binop_char_ctxe input 
+         (brackets_char input '(' parse_ast ')' )
+         token_star
+         (space_ctx input parse_ast)
+         (fun left right -> Mul (Paren left) right));
+      // n + ast
+      (binop_char_ctx input 
+         parse_number token_plus 
+         (space_ctx input parse_ast)
+         (fun left right -> Add left right));
+      // n * ast
+      (binop_char_ctx input 
+         parse_number token_star
+         (space_ctx input parse_ast)
+         (fun left right -> Mul left right));
+      // (ast)   -- should only match at end?
+      (parse_apply_ctxe 
+        input
+        (fun z -> Paren z) 
+        (brackets_char input '(' parse_ast ')' ));
+      parse_number 
+    ]
+    input
+
+let parse_or_report_fail (x:(parser ast)) : ML unit =
   let line = input_line() in 
   match x line with
-  | Success tok _ _ -> print_string ("parsed '" ^ tok ^ "'\n" )
+  | Success tree _ _ -> print_string "parsed!\n"; print_ast "" tree
   | ParseError expected at -> print_string( "expecting " ^ expected ^ " at '" ^ at ^ "'\n")
 
-let _ = parse_recursive <: parser string
-  
-let _ = parse_or_report_fail parse_recursive  
+let _ = parse_or_report_fail parse_ast
 
 (*
-let rec parse_ast (input:string) : Tot (parse_result ast input) (decreases (strlen input)) =
-  parse_either
-    (parse_literal )
-    (brackets "(" parse_ast ")" )
-    input
-  *)
   
   (*
   <|>
